store/client_proofs/connect.v
@@ -4,7 +4,8 @@ From stdpp Require Import namespaces.
 From iris.algebra Require Import agree auth csum gset gmap excl frac.
 From iris.algebra Require Import max_prefix_list.
 From iris.heap_lang Require Import notation proofmode.
-From cryptis Require Import lib version term cryptis primitives tactics.
+From cryptis Require Import lib version term gmeta nown.
+From cryptis Require Import cryptis primitives tactics.
 From cryptis Require Import role dh_auth.
 From cryptis.store Require Import impl shared db.
 From cryptis.store.client_proofs Require Import common.
@@ -48,11 +49,11 @@ iIntros "!> %Φ hon post". rewrite /Client.connect. wp_pures.
 iCombine "hon post" as "post". iRevert "post".
 iApply wp_do_until. iIntros "!> [hon post]". wp_pures.
 wp_bind (initiator _ _ _ _ _).
-iMod DB.alloc as "(%γ & auth & free & #frag)". wp_pures.
-iApply (wp_initiator γ with "[//] [//] [//] [] [] [hon]"); try solve_ndisj; eauto.
+iApply (wp_initiator with "[//] [//] [//] [] [] [hon]"); try solve_ndisj; eauto.
 iIntros "!> %okS (hon & HokS)".
 case: okS => [kS|]; wp_pures; last by iLeft; iFrame; eauto.
-iDestruct "HokS" as "(#s_kS & #sessI & #key)".
+iDestruct "HokS" as "(%γ & #s_kS & #sessI & token & #key)".
+iMod (DB.alloc with "token") as "(auth & free & #frag & token)" => //.
 wp_alloc timestamp as "ts". wp_pures.
 wp_tsenc. wp_bind (send _ _).
 iApply (wp_send with "[#] [#]") => //.
